src/EvalExecs/Transfer.v
@@ -1,0 +1,70 @@
+Require Import UrsusEnvironment.Solidity.current.Environment.
+Require Import UrsusEnvironment.Solidity.current.LocalGenerator.
+
+Require Import UMLang.ExecGenerator.
+
+Require Import EIP20.
+Import EIP20.
+
+#[global, program]
+Instance listInfinite : listInfiniteFunRec_gen XList.
+Next Obligation.
+(* TODO: we need to analyze all while/for cycles
+   and find upper bound for number of iterations *)
+exact (repeat PhantomPoint 0).
+Defined.
+
+Notation rec := LocalStateLRecord.
+
+Definition computed : LocalStateLRecord := Eval vm_compute in default. 
+#[global]
+Instance def : XDefault LocalStateLRecord := {
+  default := computed 
+} . 
+
+Definition VMStateDefault : VMStateLRecord  := Eval vm_compute in default.
+Definition LedgerDefault : LedgerLRecord LocalStateLRecord  := Eval vm_compute in default. 
+
+Elpi Accumulate rec_def lp:{{
+  get_rec {{ rec }}.
+  get_def {{ def }}.
+}}.
+
+(* Definition msg_pubkey_right (rec: Type) (def: XDefault rec) := msg_pubkey.
+
+Check  msg_sender.
+
+Definition msg_sender_right (rec: Type) (def: XDefault rec) := msg_sender.
+Check  msg_sender_right.
+
+
+Definition msg_value_right (rec: Type) (def: XDefault rec) := msg_value.
+Definition tvm_pubkey_right (rec: Type) (def: XDefault rec) := tvm_pubkey.
+Definition _now_right (rec: Type) (def: XDefault rec) := \\ now \\.
+ *)
+
+Definition transfer_exec_sig (_to :  address) 
+                             (_value :  uint256) (l : LedgerLRecord rec) :
+                             {t | t = exec_state (Uinterpreter (@transfer rec def _ _ _ _  _to _value)) l}.
+  unfold transfer. unfold dynamicAssignL.  
+  repeat auto_build_P listInfinite.
+Defined.
+
+Definition transfer_exec_let (_to :  address) 
+                             (_value :  uint256) (l : LedgerLRecord rec) : LedgerLRecord rec.
+  let_term_of_2 @transfer_exec_sig (transfer_exec_sig _to _value l).
+Defined.
+
+(* Print constructor_exec_let. *)
+
+Definition transfer_exec (_to :  address) 
+                         (_value :  uint256)  (l : LedgerLRecord rec) : LedgerLRecord rec.
+  flat_term_of_2 @transfer_exec_let (transfer_exec_let _to _value l).
+Defined.
+
+Definition transfer_prf (_to :  address) 
+                         (_value :  uint256) (l : LedgerLRecord rec) :
+  transfer_exec _to _value l = 
+  exec_state (Uinterpreter (@transfer rec def _ _ _ _ _to _value)) l.
+  proof_of_2 transfer_exec transfer_exec_sig (transfer_exec_sig _to _value l).
+Defined.
