src/Proofs/Constructor.v
@@ -1,0 +1,143 @@
+Require Import UrsusEnvironment.Solidity.current.Environment.
+Require Import UrsusEnvironment.Solidity.current.LocalGenerator.
+Require Import FinProof.Lib.HMapList.
+
+Require Import UMLang.ExecGenerator.
+
+Require Import EIP20.
+Import EIP20.
+
+Require Import EvalExecs.Constructor.
+
+#[local]
+Existing Instance BoolEq.pair_eqb_spec.
+
+
+#[global, program]
+Instance listInfinite : listInfiniteFunRec_gen XList.
+Next Obligation.
+(* TODO: we need to analyze all while/for cycles
+   and find upper bound for number of iterations *)
+exact (repeat PhantomPoint 0).
+Defined.
+
+Notation rec := LocalStateLRecord.
+
+Definition computed : LocalStateLRecord := Eval vm_compute in default. 
+#[global]
+Instance def : XDefault LocalStateLRecord := {
+  default := computed 
+} . 
+
+Definition VMStateDefault : VMStateLRecord  := Eval vm_compute in default.
+Definition LedgerDefault : LedgerLRecord LocalStateLRecord  := Eval vm_compute in default. 
+
+Elpi Accumulate rec_def lp:{{
+  get_rec {{ rec }}.
+  get_def {{ def }}.
+}}.
+
+(* Definition msg_pubkey_right (rec: Type) (def: XDefault rec) := msg_pubkey.
+
+Check  msg_sender.
+
+Definition msg_sender_right (rec: Type) (def: XDefault rec) := msg_sender.
+Check  msg_sender_right.
+
+
+Definition msg_value_right (rec: Type) (def: XDefault rec) := msg_value.
+Definition tvm_pubkey_right (rec: Type) (def: XDefault rec) := tvm_pubkey.
+Definition _now_right (rec: Type) (def: XDefault rec) := \\ now \\.
+ *)
+
+
+Lemma constructor_set__initialAmount: forall (_initialAmount :  uint256) 
+                            (_tokenName :  string) 
+                            (_decimalUnits :  uint8) 
+                            (_tokenSymbol :  string)
+                            (vmstate: VMStateLRecord), 
+    let l0 := {$$ default with Ledger_VMState := vmstate $$} in
+    let l' := exec_state (Uinterpreter (@constructor rec def _ _ _ _initialAmount _tokenName _decimalUnits _tokenSymbol)) l0 in
+    _totalSupply (l'.(Ledger_MainState)) = _initialAmount.
+Proof.
+    intros. subst l'.
+    rewrite <- constructor_prf.
+    auto.
+Qed.
+
+Lemma constructor_set__tokenName: forall (_initialAmount :  uint256) 
+                            (_tokenName :  string) 
+                            (_decimalUnits :  uint8) 
+                            (_tokenSymbol :  string)
+                            (vmstate: VMStateLRecord), 
+    let l0 := {$$ default with Ledger_VMState := vmstate $$} in                            
+    let l' := exec_state (Uinterpreter (@constructor rec def _ _ _ _initialAmount _tokenName _decimalUnits _tokenSymbol)) l0 in
+    _name (l'.(Ledger_MainState)) = _tokenName.
+Proof.
+    intros. subst l'.
+    rewrite <- constructor_prf.
+    auto.
+Qed.
+
+Lemma constructor_set__decimalUnits: forall (_initialAmount :  uint256) 
+                            (_tokenName :  string) 
+                            (_decimalUnits :  uint8) 
+                            (_tokenSymbol :  string)
+                            (vmstate: VMStateLRecord), 
+    let l0 := {$$ default with Ledger_VMState := vmstate $$} in                                
+    let l' := exec_state (Uinterpreter (@constructor rec def _ _ _ _initialAmount _tokenName _decimalUnits _tokenSymbol)) l0 in
+    _decimals (l'.(Ledger_MainState)) = _decimalUnits.
+Proof.
+    intros. subst l'.
+    rewrite <- constructor_prf.
+    auto.
+Qed.
+
+Lemma constructor_set__tokenSymbol: forall (_initialAmount :  uint256) 
+                            (_tokenName :  string) 
+                            (_decimalUnits :  uint8) 
+                            (_tokenSymbol :  string)
+                            (vmstate: VMStateLRecord), 
+    let l0 := {$$ default with Ledger_VMState := vmstate $$} in 
+    let l' := exec_state (Uinterpreter (@constructor rec def _ _ _ _initialAmount _tokenName _decimalUnits _tokenSymbol)) l0 in
+    _symbol (l'.(Ledger_MainState)) = _tokenSymbol.
+Proof.
+    intros. subst l'.
+    rewrite <- constructor_prf.
+    auto.
+Qed.
+
+
+
+Lemma constructor_set_sender_balance: forall (_initialAmount :  uint256) 
+                            (_tokenName :  string) 
+                            (_decimalUnits :  uint8) 
+                            (_tokenSymbol :  string)
+                            (l: LedgerLRecord rec),
+                            (* (vmstate: VMStateLRecord),  *)
+    let l0 := {$$ l with Ledger_LocalState := default $$} in
+    let l' := exec_state (Uinterpreter (@constructor rec def _ _ _ _initialAmount _tokenName _decimalUnits _tokenSymbol)) l0 in
+    let msg_sender := VMState_ι_msg_sender (l.(Ledger_VMState)) in
+    (_balances (l'.(Ledger_MainState))) [msg_sender] = _initialAmount.
+Proof.
+    intros. subst l'.
+    rewrite <- constructor_prf.
+
+    destruct l. repeat destruct p.
+    destruct v. repeat destruct p.
+    destruct c. repeat destruct p.
+
+    Opaque Common.hmapFindWithDefault
+           CommonInstances.addAdjustListPair.
+
+    compute.
+
+    Transparent Common.hmapFindWithDefault
+                CommonInstances.addAdjustListPair.
+
+    rewrite lookup_some_find with (v:=_initialAmount).
+    reflexivity.
+    
+    unshelve eapply lookup_addAdjust.
+    refine (BoolEq.pair_eqb_spec (X:=Z) (Y:=XUBInteger 256)).
+Qed.
